CertiGC/gc_correct.v
@@ -8,7 +8,7 @@ Require Import VST.veric.val_lemmas.
 Require Import VST.veric.shares.
 Require Import VST.msl.seplog.
 Require Import VST.msl.shares.
-Require Import VST.floyd.sublist.
+Require Import VST.zlist.sublist.
 Require Import VST.floyd.coqlib3.
 Require Import VST.floyd.functional_base.
 Require Import VST.floyd.data_at_rec_lemmas.
