kruskal/kruskal_edgelist.v
@@ -1,130 +1,137 @@
 From Coq Require Import String List ZArith.
 From compcert Require Import Coqlib Integers Floats AST Ctypes Cop Clight Clightdefs.
+Import Clightdefs.ClightNotations.
 Local Open Scope Z_scope.
+Local Open Scope string_scope.
+Local Open Scope clight_scope.
 
 Module Info.
-  Definition version := "3.7"%string.
-  Definition build_number := ""%string.
-  Definition build_tag := ""%string.
-  Definition arch := "x86"%string.
-  Definition model := "32sse2"%string.
-  Definition abi := "standard"%string.
-  Definition bitsize := 32.
+  Definition version := "3.10".
+  Definition build_number := "".
+  Definition build_tag := "".
+  Definition build_branch := "".
+  Definition arch := "x86".
+  Definition model := "64".
+  Definition abi := "standard".
+  Definition bitsize := 64.
   Definition big_endian := false.
-  Definition source_file := "kruskal/kruskal_edgelist.c"%string.
+  Definition source_file := "kruskal/kruskal_edgelist.c".
   Definition normalized := true.
 End Info.
 
-Definition _E : ident := 79%positive.
-Definition _MAX_EDGES : ident := 82%positive.
-Definition _Union : ident := 69%positive.
-Definition _V : ident := 70%positive.
-Definition ___builtin_ais_annot : ident := 4%positive.
-Definition ___builtin_annot : ident := 13%positive.
-Definition ___builtin_annot_intval : ident := 14%positive.
-Definition ___builtin_bswap : ident := 6%positive.
-Definition ___builtin_bswap16 : ident := 8%positive.
-Definition ___builtin_bswap32 : ident := 7%positive.
-Definition ___builtin_bswap64 : ident := 5%positive.
-Definition ___builtin_clz : ident := 39%positive.
-Definition ___builtin_clzl : ident := 40%positive.
-Definition ___builtin_clzll : ident := 41%positive.
-Definition ___builtin_ctz : ident := 42%positive.
-Definition ___builtin_ctzl : ident := 43%positive.
-Definition ___builtin_ctzll : ident := 44%positive.
-Definition ___builtin_debug : ident := 55%positive.
-Definition ___builtin_fabs : ident := 9%positive.
-Definition ___builtin_fmadd : ident := 47%positive.
-Definition ___builtin_fmax : ident := 45%positive.
-Definition ___builtin_fmin : ident := 46%positive.
-Definition ___builtin_fmsub : ident := 48%positive.
-Definition ___builtin_fnmadd : ident := 49%positive.
-Definition ___builtin_fnmsub : ident := 50%positive.
-Definition ___builtin_fsqrt : ident := 10%positive.
-Definition ___builtin_membar : ident := 15%positive.
-Definition ___builtin_memcpy_aligned : ident := 11%positive.
-Definition ___builtin_read16_reversed : ident := 51%positive.
-Definition ___builtin_read32_reversed : ident := 52%positive.
-Definition ___builtin_sel : ident := 12%positive.
-Definition ___builtin_va_arg : ident := 17%positive.
-Definition ___builtin_va_copy : ident := 18%positive.
-Definition ___builtin_va_end : ident := 19%positive.
-Definition ___builtin_va_start : ident := 16%positive.
-Definition ___builtin_write16_reversed : ident := 53%positive.
-Definition ___builtin_write32_reversed : ident := 54%positive.
-Definition ___compcert_i64_dtos : ident := 24%positive.
-Definition ___compcert_i64_dtou : ident := 25%positive.
-Definition ___compcert_i64_sar : ident := 36%positive.
-Definition ___compcert_i64_sdiv : ident := 30%positive.
-Definition ___compcert_i64_shl : ident := 34%positive.
-Definition ___compcert_i64_shr : ident := 35%positive.
-Definition ___compcert_i64_smod : ident := 32%positive.
-Definition ___compcert_i64_smulh : ident := 37%positive.
-Definition ___compcert_i64_stod : ident := 26%positive.
-Definition ___compcert_i64_stof : ident := 28%positive.
-Definition ___compcert_i64_udiv : ident := 31%positive.
-Definition ___compcert_i64_umod : ident := 33%positive.
-Definition ___compcert_i64_umulh : ident := 38%positive.
-Definition ___compcert_i64_utod : ident := 27%positive.
-Definition ___compcert_i64_utof : ident := 29%positive.
-Definition ___compcert_va_composite : ident := 23%positive.
-Definition ___compcert_va_float64 : ident := 22%positive.
-Definition ___compcert_va_int32 : ident := 20%positive.
-Definition ___compcert_va_int64 : ident := 21%positive.
-Definition _dst : ident := 77%positive.
-Definition _edge : ident := 78%positive.
-Definition _edge_list : ident := 80%positive.
-Definition _empty_graph : ident := 85%positive.
-Definition _fill_edge : ident := 90%positive.
-Definition _find : ident := 62%positive.
-Definition _free : ident := 84%positive.
-Definition _freeN : ident := 57%positive.
-Definition _freeSet : ident := 73%positive.
-Definition _free_graph : ident := 93%positive.
-Definition _graph : ident := 81%positive.
-Definition _graph_E : ident := 95%positive.
-Definition _graph_V : ident := 94%positive.
-Definition _graph__1 : ident := 92%positive.
-Definition _i : ident := 59%positive.
-Definition _init_empty_graph : ident := 86%positive.
-Definition _kruskal : ident := 99%positive.
-Definition _main : ident := 74%positive.
-Definition _makeSet : ident := 72%positive.
-Definition _mallocK : ident := 83%positive.
-Definition _mallocN : ident := 56%positive.
-Definition _mst : ident := 96%positive.
-Definition _p : ident := 61%positive.
-Definition _p0 : ident := 60%positive.
-Definition _parent : ident := 1%positive.
-Definition _rank : ident := 2%positive.
-Definition _sort_edges : ident := 91%positive.
-Definition _src : ident := 76%positive.
-Definition _subset : ident := 3%positive.
-Definition _subsets : ident := 58%positive.
-Definition _u : ident := 89%positive.
-Definition _ufind : ident := 97%positive.
-Definition _v : ident := 71%positive.
-Definition _vfind : ident := 98%positive.
-Definition _w : ident := 88%positive.
-Definition _wedge : ident := 87%positive.
-Definition _weight : ident := 75%positive.
-Definition _x : ident := 63%positive.
-Definition _xRank : ident := 67%positive.
-Definition _xroot : ident := 65%positive.
-Definition _y : ident := 64%positive.
-Definition _yRank : ident := 68%positive.
-Definition _yroot : ident := 66%positive.
-Definition _t'1 : ident := 100%positive.
-Definition _t'10 : ident := 109%positive.
-Definition _t'11 : ident := 110%positive.
-Definition _t'2 : ident := 101%positive.
-Definition _t'3 : ident := 102%positive.
-Definition _t'4 : ident := 103%positive.
-Definition _t'5 : ident := 104%positive.
-Definition _t'6 : ident := 105%positive.
-Definition _t'7 : ident := 106%positive.
-Definition _t'8 : ident := 107%positive.
-Definition _t'9 : ident := 108%positive.
+Definition _E : ident := $"E".
+Definition _MAX_EDGES : ident := $"MAX_EDGES".
+Definition _Union : ident := $"Union".
+Definition _V : ident := $"V".
+Definition ___builtin_annot : ident := $"__builtin_annot".
+Definition ___builtin_annot_intval : ident := $"__builtin_annot_intval".
+Definition ___builtin_bswap : ident := $"__builtin_bswap".
+Definition ___builtin_bswap16 : ident := $"__builtin_bswap16".
+Definition ___builtin_bswap32 : ident := $"__builtin_bswap32".
+Definition ___builtin_bswap64 : ident := $"__builtin_bswap64".
+Definition ___builtin_clz : ident := $"__builtin_clz".
+Definition ___builtin_clzl : ident := $"__builtin_clzl".
+Definition ___builtin_clzll : ident := $"__builtin_clzll".
+Definition ___builtin_ctz : ident := $"__builtin_ctz".
+Definition ___builtin_ctzl : ident := $"__builtin_ctzl".
+Definition ___builtin_ctzll : ident := $"__builtin_ctzll".
+Definition ___builtin_debug : ident := $"__builtin_debug".
+Definition ___builtin_expect : ident := $"__builtin_expect".
+Definition ___builtin_fabs : ident := $"__builtin_fabs".
+Definition ___builtin_fabsf : ident := $"__builtin_fabsf".
+Definition ___builtin_fmadd : ident := $"__builtin_fmadd".
+Definition ___builtin_fmax : ident := $"__builtin_fmax".
+Definition ___builtin_fmin : ident := $"__builtin_fmin".
+Definition ___builtin_fmsub : ident := $"__builtin_fmsub".
+Definition ___builtin_fnmadd : ident := $"__builtin_fnmadd".
+Definition ___builtin_fnmsub : ident := $"__builtin_fnmsub".
+Definition ___builtin_fsqrt : ident := $"__builtin_fsqrt".
+Definition ___builtin_membar : ident := $"__builtin_membar".
+Definition ___builtin_memcpy_aligned : ident := $"__builtin_memcpy_aligned".
+Definition ___builtin_read16_reversed : ident := $"__builtin_read16_reversed".
+Definition ___builtin_read32_reversed : ident := $"__builtin_read32_reversed".
+Definition ___builtin_sel : ident := $"__builtin_sel".
+Definition ___builtin_sqrt : ident := $"__builtin_sqrt".
+Definition ___builtin_unreachable : ident := $"__builtin_unreachable".
+Definition ___builtin_va_arg : ident := $"__builtin_va_arg".
+Definition ___builtin_va_copy : ident := $"__builtin_va_copy".
+Definition ___builtin_va_end : ident := $"__builtin_va_end".
+Definition ___builtin_va_start : ident := $"__builtin_va_start".
+Definition ___builtin_write16_reversed : ident := $"__builtin_write16_reversed".
+Definition ___builtin_write32_reversed : ident := $"__builtin_write32_reversed".
+Definition ___compcert_i64_dtos : ident := $"__compcert_i64_dtos".
+Definition ___compcert_i64_dtou : ident := $"__compcert_i64_dtou".
+Definition ___compcert_i64_sar : ident := $"__compcert_i64_sar".
+Definition ___compcert_i64_sdiv : ident := $"__compcert_i64_sdiv".
+Definition ___compcert_i64_shl : ident := $"__compcert_i64_shl".
+Definition ___compcert_i64_shr : ident := $"__compcert_i64_shr".
+Definition ___compcert_i64_smod : ident := $"__compcert_i64_smod".
+Definition ___compcert_i64_smulh : ident := $"__compcert_i64_smulh".
+Definition ___compcert_i64_stod : ident := $"__compcert_i64_stod".
+Definition ___compcert_i64_stof : ident := $"__compcert_i64_stof".
+Definition ___compcert_i64_udiv : ident := $"__compcert_i64_udiv".
+Definition ___compcert_i64_umod : ident := $"__compcert_i64_umod".
+Definition ___compcert_i64_umulh : ident := $"__compcert_i64_umulh".
+Definition ___compcert_i64_utod : ident := $"__compcert_i64_utod".
+Definition ___compcert_i64_utof : ident := $"__compcert_i64_utof".
+Definition ___compcert_va_composite : ident := $"__compcert_va_composite".
+Definition ___compcert_va_float64 : ident := $"__compcert_va_float64".
+Definition ___compcert_va_int32 : ident := $"__compcert_va_int32".
+Definition ___compcert_va_int64 : ident := $"__compcert_va_int64".
+Definition _dst : ident := $"dst".
+Definition _edge : ident := $"edge".
+Definition _edge_list : ident := $"edge_list".
+Definition _empty_graph : ident := $"empty_graph".
+Definition _fill_edge : ident := $"fill_edge".
+Definition _find : ident := $"find".
+Definition _free : ident := $"free".
+Definition _freeN : ident := $"freeN".
+Definition _freeSet : ident := $"freeSet".
+Definition _free_graph : ident := $"free_graph".
+Definition _graph : ident := $"graph".
+Definition _graph_E : ident := $"graph_E".
+Definition _graph_V : ident := $"graph_V".
+Definition _graph__1 : ident := $"graph__1".
+Definition _i : ident := $"i".
+Definition _init_empty_graph : ident := $"init_empty_graph".
+Definition _kruskal : ident := $"kruskal".
+Definition _main : ident := $"main".
+Definition _makeSet : ident := $"makeSet".
+Definition _mallocK : ident := $"mallocK".
+Definition _mallocN : ident := $"mallocN".
+Definition _mst : ident := $"mst".
+Definition _p : ident := $"p".
+Definition _p0 : ident := $"p0".
+Definition _parent : ident := $"parent".
+Definition _rank : ident := $"rank".
+Definition _sort_edges : ident := $"sort_edges".
+Definition _src : ident := $"src".
+Definition _subset : ident := $"subset".
+Definition _subsets : ident := $"subsets".
+Definition _u : ident := $"u".
+Definition _ufind : ident := $"ufind".
+Definition _v : ident := $"v".
+Definition _vfind : ident := $"vfind".
+Definition _w : ident := $"w".
+Definition _wedge : ident := $"wedge".
+Definition _weight : ident := $"weight".
+Definition _x : ident := $"x".
+Definition _xRank : ident := $"xRank".
+Definition _xroot : ident := $"xroot".
+Definition _y : ident := $"y".
+Definition _yRank : ident := $"yRank".
+Definition _yroot : ident := $"yroot".
+Definition _t'1 : ident := 128%positive.
+Definition _t'10 : ident := 137%positive.
+Definition _t'11 : ident := 138%positive.
+Definition _t'2 : ident := 129%positive.
+Definition _t'3 : ident := 130%positive.
+Definition _t'4 : ident := 131%positive.
+Definition _t'5 : ident := 132%positive.
+Definition _t'6 : ident := 133%positive.
+Definition _t'7 : ident := 134%positive.
+Definition _t'8 : ident := 135%positive.
+Definition _t'9 : ident := 136%positive.
 
 Definition v_MAX_EDGES := {|
   gvar_info := tint;
@@ -147,7 +154,7 @@ Definition f_init_empty_graph := {|
   (Ssequence
     (Scall (Some _t'1)
       (Evar _mallocK (Tfunction (Tcons tint Tnil) (tptr tvoid) cc_default))
-      ((Esizeof (Tstruct _graph noattr) tuint) :: nil))
+      ((Esizeof (Tstruct _graph noattr) tulong) :: nil))
     (Sset _empty_graph
       (Ecast (Etempvar _t'1 (tptr tvoid)) (tptr (Tstruct _graph noattr)))))
   (Ssequence
@@ -157,8 +164,8 @@ Definition f_init_empty_graph := {|
         (Scall (Some _t'2)
           (Evar _mallocK (Tfunction (Tcons tint Tnil) (tptr tvoid)
                            cc_default))
-          ((Ebinop Omul (Esizeof (Tstruct _edge noattr) tuint)
-             (Etempvar _t'3 tint) tuint) :: nil)))
+          ((Ebinop Omul (Esizeof (Tstruct _edge noattr) tulong)
+             (Etempvar _t'3 tint) tulong) :: nil)))
       (Sset _edge_list
         (Ecast (Etempvar _t'2 (tptr tvoid)) (tptr (Tstruct _edge noattr)))))
     (Ssequence
@@ -438,109 +445,35 @@ Definition f_kruskal := {|
 |}.
 
 Definition composites : list composite_definition :=
-(Composite _subset Struct ((_parent, tint) :: (_rank, tuint) :: nil) noattr ::
+(Composite _subset Struct
+   (Member_plain _parent tint :: Member_plain _rank tuint :: nil)
+   noattr ::
  Composite _edge Struct
-   ((_weight, tint) :: (_src, tint) :: (_dst, tint) :: nil)
+   (Member_plain _weight tint :: Member_plain _src tint ::
+    Member_plain _dst tint :: nil)
    noattr ::
  Composite _graph Struct
-   ((_V, tint) :: (_E, tint) ::
-    (_edge_list, (tptr (Tstruct _edge noattr))) :: nil)
+   (Member_plain _V tint :: Member_plain _E tint ::
+    Member_plain _edge_list (tptr (Tstruct _edge noattr)) :: nil)
    noattr :: nil).
 
 Definition global_definitions : list (ident * globdef fundef type) :=
-((___builtin_ais_annot,
-   Gfun(External (EF_builtin "__builtin_ais_annot"
-                   (mksignature (AST.Tint :: nil) AST.Tvoid
-                     {|cc_vararg:=true; cc_unproto:=false; cc_structret:=false|}))
-     (Tcons (tptr tschar) Tnil) tvoid
-     {|cc_vararg:=true; cc_unproto:=false; cc_structret:=false|})) ::
- (___builtin_bswap64,
-   Gfun(External (EF_builtin "__builtin_bswap64"
-                   (mksignature (AST.Tlong :: nil) AST.Tlong cc_default))
-     (Tcons tulong Tnil) tulong cc_default)) ::
- (___builtin_bswap,
-   Gfun(External (EF_builtin "__builtin_bswap"
-                   (mksignature (AST.Tint :: nil) AST.Tint cc_default))
-     (Tcons tuint Tnil) tuint cc_default)) ::
- (___builtin_bswap32,
-   Gfun(External (EF_builtin "__builtin_bswap32"
-                   (mksignature (AST.Tint :: nil) AST.Tint cc_default))
-     (Tcons tuint Tnil) tuint cc_default)) ::
- (___builtin_bswap16,
-   Gfun(External (EF_builtin "__builtin_bswap16"
-                   (mksignature (AST.Tint :: nil) AST.Tint16unsigned
-                     cc_default)) (Tcons tushort Tnil) tushort cc_default)) ::
- (___builtin_fabs,
-   Gfun(External (EF_builtin "__builtin_fabs"
-                   (mksignature (AST.Tfloat :: nil) AST.Tfloat cc_default))
-     (Tcons tdouble Tnil) tdouble cc_default)) ::
- (___builtin_fsqrt,
-   Gfun(External (EF_builtin "__builtin_fsqrt"
-                   (mksignature (AST.Tfloat :: nil) AST.Tfloat cc_default))
-     (Tcons tdouble Tnil) tdouble cc_default)) ::
- (___builtin_memcpy_aligned,
-   Gfun(External (EF_builtin "__builtin_memcpy_aligned"
-                   (mksignature
-                     (AST.Tint :: AST.Tint :: AST.Tint :: AST.Tint :: nil)
-                     AST.Tvoid cc_default))
-     (Tcons (tptr tvoid)
-       (Tcons (tptr tvoid) (Tcons tuint (Tcons tuint Tnil)))) tvoid
-     cc_default)) ::
- (___builtin_sel,
-   Gfun(External (EF_builtin "__builtin_sel"
-                   (mksignature (AST.Tint :: nil) AST.Tvoid
-                     {|cc_vararg:=true; cc_unproto:=false; cc_structret:=false|}))
-     (Tcons tbool Tnil) tvoid
-     {|cc_vararg:=true; cc_unproto:=false; cc_structret:=false|})) ::
- (___builtin_annot,
-   Gfun(External (EF_builtin "__builtin_annot"
-                   (mksignature (AST.Tint :: nil) AST.Tvoid
-                     {|cc_vararg:=true; cc_unproto:=false; cc_structret:=false|}))
-     (Tcons (tptr tschar) Tnil) tvoid
-     {|cc_vararg:=true; cc_unproto:=false; cc_structret:=false|})) ::
- (___builtin_annot_intval,
-   Gfun(External (EF_builtin "__builtin_annot_intval"
-                   (mksignature (AST.Tint :: AST.Tint :: nil) AST.Tint
-                     cc_default)) (Tcons (tptr tschar) (Tcons tint Tnil))
-     tint cc_default)) ::
- (___builtin_membar,
-   Gfun(External (EF_builtin "__builtin_membar"
-                   (mksignature nil AST.Tvoid cc_default)) Tnil tvoid
-     cc_default)) ::
- (___builtin_va_start,
-   Gfun(External (EF_builtin "__builtin_va_start"
-                   (mksignature (AST.Tint :: nil) AST.Tvoid cc_default))
-     (Tcons (tptr tvoid) Tnil) tvoid cc_default)) ::
- (___builtin_va_arg,
-   Gfun(External (EF_builtin "__builtin_va_arg"
-                   (mksignature (AST.Tint :: AST.Tint :: nil) AST.Tvoid
-                     cc_default)) (Tcons (tptr tvoid) (Tcons tuint Tnil))
-     tvoid cc_default)) ::
- (___builtin_va_copy,
-   Gfun(External (EF_builtin "__builtin_va_copy"
-                   (mksignature (AST.Tint :: AST.Tint :: nil) AST.Tvoid
-                     cc_default))
-     (Tcons (tptr tvoid) (Tcons (tptr tvoid) Tnil)) tvoid cc_default)) ::
- (___builtin_va_end,
-   Gfun(External (EF_builtin "__builtin_va_end"
-                   (mksignature (AST.Tint :: nil) AST.Tvoid cc_default))
-     (Tcons (tptr tvoid) Tnil) tvoid cc_default)) ::
- (___compcert_va_int32,
-   Gfun(External (EF_external "__compcert_va_int32"
-                   (mksignature (AST.Tint :: nil) AST.Tint cc_default))
+((___compcert_va_int32,
+   Gfun(External (EF_runtime "__compcert_va_int32"
+                   (mksignature (AST.Tlong :: nil) AST.Tint cc_default))
      (Tcons (tptr tvoid) Tnil) tuint cc_default)) ::
  (___compcert_va_int64,
-   Gfun(External (EF_external "__compcert_va_int64"
-                   (mksignature (AST.Tint :: nil) AST.Tlong cc_default))
+   Gfun(External (EF_runtime "__compcert_va_int64"
+                   (mksignature (AST.Tlong :: nil) AST.Tlong cc_default))
      (Tcons (tptr tvoid) Tnil) tulong cc_default)) ::
  (___compcert_va_float64,
-   Gfun(External (EF_external "__compcert_va_float64"
-                   (mksignature (AST.Tint :: nil) AST.Tfloat cc_default))
+   Gfun(External (EF_runtime "__compcert_va_float64"
+                   (mksignature (AST.Tlong :: nil) AST.Tfloat cc_default))
      (Tcons (tptr tvoid) Tnil) tdouble cc_default)) ::
  (___compcert_va_composite,
-   Gfun(External (EF_external "__compcert_va_composite"
-                   (mksignature (AST.Tint :: AST.Tint :: nil) AST.Tint
-                     cc_default)) (Tcons (tptr tvoid) (Tcons tuint Tnil))
+   Gfun(External (EF_runtime "__compcert_va_composite"
+                   (mksignature (AST.Tlong :: AST.Tlong :: nil) AST.Tlong
+                     cc_default)) (Tcons (tptr tvoid) (Tcons tulong Tnil))
      (tptr tvoid) cc_default)) ::
  (___compcert_i64_dtos,
    Gfun(External (EF_runtime "__compcert_i64_dtos"
@@ -611,14 +544,30 @@ Definition global_definitions : list (ident * globdef fundef type) :=
                    (mksignature (AST.Tlong :: AST.Tlong :: nil) AST.Tlong
                      cc_default)) (Tcons tulong (Tcons tulong Tnil)) tulong
      cc_default)) ::
+ (___builtin_bswap64,
+   Gfun(External (EF_builtin "__builtin_bswap64"
+                   (mksignature (AST.Tlong :: nil) AST.Tlong cc_default))
+     (Tcons tulong Tnil) tulong cc_default)) ::
+ (___builtin_bswap,
+   Gfun(External (EF_builtin "__builtin_bswap"
+                   (mksignature (AST.Tint :: nil) AST.Tint cc_default))
+     (Tcons tuint Tnil) tuint cc_default)) ::
+ (___builtin_bswap32,
+   Gfun(External (EF_builtin "__builtin_bswap32"
+                   (mksignature (AST.Tint :: nil) AST.Tint cc_default))
+     (Tcons tuint Tnil) tuint cc_default)) ::
+ (___builtin_bswap16,
+   Gfun(External (EF_builtin "__builtin_bswap16"
+                   (mksignature (AST.Tint :: nil) AST.Tint16unsigned
+                     cc_default)) (Tcons tushort Tnil) tushort cc_default)) ::
  (___builtin_clz,
    Gfun(External (EF_builtin "__builtin_clz"
                    (mksignature (AST.Tint :: nil) AST.Tint cc_default))
      (Tcons tuint Tnil) tint cc_default)) ::
  (___builtin_clzl,
    Gfun(External (EF_builtin "__builtin_clzl"
-                   (mksignature (AST.Tint :: nil) AST.Tint cc_default))
-     (Tcons tuint Tnil) tint cc_default)) ::
+                   (mksignature (AST.Tlong :: nil) AST.Tint cc_default))
+     (Tcons tulong Tnil) tint cc_default)) ::
  (___builtin_clzll,
    Gfun(External (EF_builtin "__builtin_clzll"
                    (mksignature (AST.Tlong :: nil) AST.Tint cc_default))
@@ -629,12 +578,84 @@ Definition global_definitions : list (ident * globdef fundef type) :=
      (Tcons tuint Tnil) tint cc_default)) ::
  (___builtin_ctzl,
    Gfun(External (EF_builtin "__builtin_ctzl"
-                   (mksignature (AST.Tint :: nil) AST.Tint cc_default))
-     (Tcons tuint Tnil) tint cc_default)) ::
+                   (mksignature (AST.Tlong :: nil) AST.Tint cc_default))
+     (Tcons tulong Tnil) tint cc_default)) ::
  (___builtin_ctzll,
    Gfun(External (EF_builtin "__builtin_ctzll"
                    (mksignature (AST.Tlong :: nil) AST.Tint cc_default))
      (Tcons tulong Tnil) tint cc_default)) ::
+ (___builtin_fabs,
+   Gfun(External (EF_builtin "__builtin_fabs"
+                   (mksignature (AST.Tfloat :: nil) AST.Tfloat cc_default))
+     (Tcons tdouble Tnil) tdouble cc_default)) ::
+ (___builtin_fabsf,
+   Gfun(External (EF_builtin "__builtin_fabsf"
+                   (mksignature (AST.Tsingle :: nil) AST.Tsingle cc_default))
+     (Tcons tfloat Tnil) tfloat cc_default)) ::
+ (___builtin_fsqrt,
+   Gfun(External (EF_builtin "__builtin_fsqrt"
+                   (mksignature (AST.Tfloat :: nil) AST.Tfloat cc_default))
+     (Tcons tdouble Tnil) tdouble cc_default)) ::
+ (___builtin_sqrt,
+   Gfun(External (EF_builtin "__builtin_sqrt"
+                   (mksignature (AST.Tfloat :: nil) AST.Tfloat cc_default))
+     (Tcons tdouble Tnil) tdouble cc_default)) ::
+ (___builtin_memcpy_aligned,
+   Gfun(External (EF_builtin "__builtin_memcpy_aligned"
+                   (mksignature
+                     (AST.Tlong :: AST.Tlong :: AST.Tlong :: AST.Tlong ::
+                      nil) AST.Tvoid cc_default))
+     (Tcons (tptr tvoid)
+       (Tcons (tptr tvoid) (Tcons tulong (Tcons tulong Tnil)))) tvoid
+     cc_default)) ::
+ (___builtin_sel,
+   Gfun(External (EF_builtin "__builtin_sel"
+                   (mksignature (AST.Tint :: nil) AST.Tvoid
+                     {|cc_vararg:=(Some 1); cc_unproto:=false; cc_structret:=false|}))
+     (Tcons tbool Tnil) tvoid
+     {|cc_vararg:=(Some 1); cc_unproto:=false; cc_structret:=false|})) ::
+ (___builtin_annot,
+   Gfun(External (EF_builtin "__builtin_annot"
+                   (mksignature (AST.Tlong :: nil) AST.Tvoid
+                     {|cc_vararg:=(Some 1); cc_unproto:=false; cc_structret:=false|}))
+     (Tcons (tptr tschar) Tnil) tvoid
+     {|cc_vararg:=(Some 1); cc_unproto:=false; cc_structret:=false|})) ::
+ (___builtin_annot_intval,
+   Gfun(External (EF_builtin "__builtin_annot_intval"
+                   (mksignature (AST.Tlong :: AST.Tint :: nil) AST.Tint
+                     cc_default)) (Tcons (tptr tschar) (Tcons tint Tnil))
+     tint cc_default)) ::
+ (___builtin_membar,
+   Gfun(External (EF_builtin "__builtin_membar"
+                   (mksignature nil AST.Tvoid cc_default)) Tnil tvoid
+     cc_default)) ::
+ (___builtin_va_start,
+   Gfun(External (EF_builtin "__builtin_va_start"
+                   (mksignature (AST.Tlong :: nil) AST.Tvoid cc_default))
+     (Tcons (tptr tvoid) Tnil) tvoid cc_default)) ::
+ (___builtin_va_arg,
+   Gfun(External (EF_builtin "__builtin_va_arg"
+                   (mksignature (AST.Tlong :: AST.Tint :: nil) AST.Tvoid
+                     cc_default)) (Tcons (tptr tvoid) (Tcons tuint Tnil))
+     tvoid cc_default)) ::
+ (___builtin_va_copy,
+   Gfun(External (EF_builtin "__builtin_va_copy"
+                   (mksignature (AST.Tlong :: AST.Tlong :: nil) AST.Tvoid
+                     cc_default))
+     (Tcons (tptr tvoid) (Tcons (tptr tvoid) Tnil)) tvoid cc_default)) ::
+ (___builtin_va_end,
+   Gfun(External (EF_builtin "__builtin_va_end"
+                   (mksignature (AST.Tlong :: nil) AST.Tvoid cc_default))
+     (Tcons (tptr tvoid) Tnil) tvoid cc_default)) ::
+ (___builtin_unreachable,
+   Gfun(External (EF_builtin "__builtin_unreachable"
+                   (mksignature nil AST.Tvoid cc_default)) Tnil tvoid
+     cc_default)) ::
+ (___builtin_expect,
+   Gfun(External (EF_builtin "__builtin_expect"
+                   (mksignature (AST.Tlong :: AST.Tlong :: nil) AST.Tlong
+                     cc_default)) (Tcons tlong (Tcons tlong Tnil)) tlong
+     cc_default)) ::
  (___builtin_fmax,
    Gfun(External (EF_builtin "__builtin_fmax"
                    (mksignature (AST.Tfloat :: AST.Tfloat :: nil) AST.Tfloat
@@ -675,60 +696,60 @@ Definition global_definitions : list (ident * globdef fundef type) :=
      cc_default)) ::
  (___builtin_read16_reversed,
    Gfun(External (EF_builtin "__builtin_read16_reversed"
-                   (mksignature (AST.Tint :: nil) AST.Tint16unsigned
+                   (mksignature (AST.Tlong :: nil) AST.Tint16unsigned
                      cc_default)) (Tcons (tptr tushort) Tnil) tushort
      cc_default)) ::
  (___builtin_read32_reversed,
    Gfun(External (EF_builtin "__builtin_read32_reversed"
-                   (mksignature (AST.Tint :: nil) AST.Tint cc_default))
+                   (mksignature (AST.Tlong :: nil) AST.Tint cc_default))
      (Tcons (tptr tuint) Tnil) tuint cc_default)) ::
  (___builtin_write16_reversed,
    Gfun(External (EF_builtin "__builtin_write16_reversed"
-                   (mksignature (AST.Tint :: AST.Tint :: nil) AST.Tvoid
+                   (mksignature (AST.Tlong :: AST.Tint :: nil) AST.Tvoid
                      cc_default)) (Tcons (tptr tushort) (Tcons tushort Tnil))
      tvoid cc_default)) ::
  (___builtin_write32_reversed,
    Gfun(External (EF_builtin "__builtin_write32_reversed"
-                   (mksignature (AST.Tint :: AST.Tint :: nil) AST.Tvoid
+                   (mksignature (AST.Tlong :: AST.Tint :: nil) AST.Tvoid
                      cc_default)) (Tcons (tptr tuint) (Tcons tuint Tnil))
      tvoid cc_default)) ::
  (___builtin_debug,
    Gfun(External (EF_external "__builtin_debug"
                    (mksignature (AST.Tint :: nil) AST.Tvoid
-                     {|cc_vararg:=true; cc_unproto:=false; cc_structret:=false|}))
+                     {|cc_vararg:=(Some 1); cc_unproto:=false; cc_structret:=false|}))
      (Tcons tint Tnil) tvoid
-     {|cc_vararg:=true; cc_unproto:=false; cc_structret:=false|})) ::
+     {|cc_vararg:=(Some 1); cc_unproto:=false; cc_structret:=false|})) ::
  (_find,
    Gfun(External (EF_external "find"
-                   (mksignature (AST.Tint :: AST.Tint :: nil) AST.Tint
+                   (mksignature (AST.Tlong :: AST.Tint :: nil) AST.Tint
                      cc_default))
      (Tcons (tptr (Tstruct _subset noattr)) (Tcons tint Tnil)) tint
      cc_default)) ::
  (_Union,
    Gfun(External (EF_external "Union"
-                   (mksignature (AST.Tint :: AST.Tint :: AST.Tint :: nil)
+                   (mksignature (AST.Tlong :: AST.Tint :: AST.Tint :: nil)
                      AST.Tvoid cc_default))
      (Tcons (tptr (Tstruct _subset noattr)) (Tcons tint (Tcons tint Tnil)))
      tvoid cc_default)) ::
  (_makeSet,
    Gfun(External (EF_external "makeSet"
-                   (mksignature (AST.Tint :: nil) AST.Tint cc_default))
+                   (mksignature (AST.Tint :: nil) AST.Tlong cc_default))
      (Tcons tint Tnil) (tptr (Tstruct _subset noattr)) cc_default)) ::
  (_freeSet,
    Gfun(External (EF_external "freeSet"
-                   (mksignature (AST.Tint :: nil) AST.Tvoid cc_default))
+                   (mksignature (AST.Tlong :: nil) AST.Tvoid cc_default))
      (Tcons (tptr (Tstruct _subset noattr)) Tnil) tvoid cc_default)) ::
  (_MAX_EDGES, Gvar v_MAX_EDGES) ::
  (_mallocK,
    Gfun(External (EF_external "mallocK"
-                   (mksignature (AST.Tint :: nil) AST.Tint cc_default))
+                   (mksignature (AST.Tint :: nil) AST.Tlong cc_default))
      (Tcons tint Tnil) (tptr tvoid) cc_default)) ::
  (_free, Gfun(External EF_free (Tcons (tptr tvoid) Tnil) tvoid cc_default)) ::
  (_init_empty_graph, Gfun(Internal f_init_empty_graph)) ::
  (_fill_edge, Gfun(Internal f_fill_edge)) ::
  (_sort_edges,
    Gfun(External (EF_external "sort_edges"
-                   (mksignature (AST.Tint :: AST.Tint :: nil) AST.Tvoid
+                   (mksignature (AST.Tlong :: AST.Tint :: nil) AST.Tvoid
                      cc_default))
      (Tcons (tptr (Tstruct _edge noattr)) (Tcons tint Tnil)) tvoid
      cc_default)) :: (_free_graph, Gfun(Internal f_free_graph)) ::
@@ -741,20 +762,22 @@ Definition public_idents : list ident :=
  ___builtin_write16_reversed :: ___builtin_read32_reversed ::
  ___builtin_read16_reversed :: ___builtin_fnmsub :: ___builtin_fnmadd ::
  ___builtin_fmsub :: ___builtin_fmadd :: ___builtin_fmin ::
- ___builtin_fmax :: ___builtin_ctzll :: ___builtin_ctzl :: ___builtin_ctz ::
+ ___builtin_fmax :: ___builtin_expect :: ___builtin_unreachable ::
+ ___builtin_va_end :: ___builtin_va_copy :: ___builtin_va_arg ::
+ ___builtin_va_start :: ___builtin_membar :: ___builtin_annot_intval ::
+ ___builtin_annot :: ___builtin_sel :: ___builtin_memcpy_aligned ::
+ ___builtin_sqrt :: ___builtin_fsqrt :: ___builtin_fabsf ::
+ ___builtin_fabs :: ___builtin_ctzll :: ___builtin_ctzl :: ___builtin_ctz ::
  ___builtin_clzll :: ___builtin_clzl :: ___builtin_clz ::
- ___compcert_i64_umulh :: ___compcert_i64_smulh :: ___compcert_i64_sar ::
- ___compcert_i64_shr :: ___compcert_i64_shl :: ___compcert_i64_umod ::
- ___compcert_i64_smod :: ___compcert_i64_udiv :: ___compcert_i64_sdiv ::
- ___compcert_i64_utof :: ___compcert_i64_stof :: ___compcert_i64_utod ::
- ___compcert_i64_stod :: ___compcert_i64_dtou :: ___compcert_i64_dtos ::
- ___compcert_va_composite :: ___compcert_va_float64 ::
- ___compcert_va_int64 :: ___compcert_va_int32 :: ___builtin_va_end ::
- ___builtin_va_copy :: ___builtin_va_arg :: ___builtin_va_start ::
- ___builtin_membar :: ___builtin_annot_intval :: ___builtin_annot ::
- ___builtin_sel :: ___builtin_memcpy_aligned :: ___builtin_fsqrt ::
- ___builtin_fabs :: ___builtin_bswap16 :: ___builtin_bswap32 ::
- ___builtin_bswap :: ___builtin_bswap64 :: ___builtin_ais_annot :: nil).
+ ___builtin_bswap16 :: ___builtin_bswap32 :: ___builtin_bswap ::
+ ___builtin_bswap64 :: ___compcert_i64_umulh :: ___compcert_i64_smulh ::
+ ___compcert_i64_sar :: ___compcert_i64_shr :: ___compcert_i64_shl ::
+ ___compcert_i64_umod :: ___compcert_i64_smod :: ___compcert_i64_udiv ::
+ ___compcert_i64_sdiv :: ___compcert_i64_utof :: ___compcert_i64_stof ::
+ ___compcert_i64_utod :: ___compcert_i64_stod :: ___compcert_i64_dtou ::
+ ___compcert_i64_dtos :: ___compcert_va_composite ::
+ ___compcert_va_float64 :: ___compcert_va_int64 :: ___compcert_va_int32 ::
+ nil).
 
 Definition prog : Clight.program := 
   mkprogram composites global_definitions public_idents _main Logic.I.
