msl_ext/alg_seplog.v
@@ -15,7 +15,7 @@ Local Open Scope logic.
 Instance algPreciseSepLog (A : Type) {JA : Join A} {PA : Perm_alg A} {SA: Sep_alg A} {AG : ageable A} {AA: Age_alg A}: PreciseSepLog (pred A).
   apply (mkPreciseSepLog precise); simpl; intros.
   (* + eapply precise_left_sepcon_andp_distr_i; eauto. *)
-  + eapply derives_precise; eauto.
+  + apply derives_precise with Q. apply H. auto.
   + apply precise_emp.
   + apply precise_sepcon_i; auto.
   (* + apply precise_wand_ewand_i; auto. *)
@@ -25,17 +25,17 @@ Instance algOverlapSepLog (A: Type) {JA: Join A} {SA: Sep_alg A} {PA : Perm_alg 
   apply (mkOverlapSepLog ocon owand); unfold algNatDed, algSepLog, algPreciseSepLog; simpl.
   + apply ocon_emp_i.
   + apply ocon_TT_i.
-  + apply andp_ocon_i.
+  + intros.  constructor. apply andp_ocon_i.
   + apply ocon_andp_prop_i.
-  + apply sepcon_ocon_i.
-  + intros. rewrite ocon_wand_i.
+  + intros.  constructor. apply sepcon_ocon_i.
+  + intros. rewrite ocon_wand_i. constructor.
     apply (exp_right R).
     apply derives_refl.
   + apply ocon_comm_i.
   + apply ocon_assoc_i.
-  + apply ocon_derives_i.
-  + apply owand_ocon_adjoint_i.
-  + apply ocon_contain_i.
+  +  constructor. inv H. inv H0. apply ocon_derives_i; auto.
+  + intros. split; intro H; inv H; constructor;  apply owand_ocon_adjoint_i; auto.
+  + intros. inv H; constructor; apply ocon_contain_i; auto.
   (* + apply precise_ocon_contain_i. *)
   + apply precise_ocon_self.
   + apply precise_ocon_i.
@@ -43,10 +43,10 @@ Defined.
 
 Instance algDisjointedSepLog (A: Type) {JA: Join A} {PA : Perm_alg A} {SA: Sep_alg A} {DA: Disj_alg A} {TA: Trip_alg A} {CrA: Cross_alg A} {AG : ageable A} {AA : Age_alg A} : DisjointedSepLog (pred A).
   apply (mkDisjointedSepLog disjointed); unfold algNatDed, algSepLog, algPreciseSepLog; simpl.
-  + apply ocon_sepcon_i.
+  + constructor; apply ocon_sepcon_i; auto.
   + apply disj_emp_i.
   + apply disj_comm_i.
-  + apply disj_derives_i.
+  + intros. inv H. inv H0. eapply disj_derives_i; eauto.
   + apply disj_ocon_right_i.
 Defined.
 
