prim/MatrixUGraph.v
@@ -1,5 +1,5 @@
 Require Import Coq.micromega.Lia.
-Require Import VST.floyd.sublist.
+Require Import VST.zlist.sublist.
 Require Import compcert.lib.Integers.
 Require Import compcert.lib.Coqlib.
 Require Import CertiGraph.lib.EquivDec_ext.
